lean/tacticComb.lean
@@ -1,0 +1,111 @@
+lemma L1 : ∀ (p q:Prop), p → p ∨ q :=
+  begin intros p q H, left, assumption end
+
+#check L1
+
+lemma L2 : ∀ (p q:Prop), p → p ∨ q :=
+  assume p q (H : p), by {left, assumption}
+
+#check L2
+
+lemma L3 : ∀ (p q:Prop), p → q → p ∧ q :=
+  assume p q Hp Hq, by {split; assumption}
+
+#check L3
+
+lemma L4 : ∀ (p q:Prop), p → p ∨ q :=
+  assume p q Hp, by {left, assumption} <|> {right, assumption}
+
+#check L4
+
+lemma L5 : ∀ (p q:Prop), q → p ∨ q :=
+  assume p q Hq, by {left, assumption} <|> {right, assumption}
+
+#check L5
+
+
+lemma L6 : ∀ (p q r:Prop), p → p ∨ q ∨ r :=
+  assume p q r H, by repeat {{left, assumption} <|> right <|> assumption}
+
+#check L6
+
+
+lemma L7 : ∀ (p q r:Prop), q → p ∨ q ∨ r :=
+  assume p q r H, by repeat {{left, assumption} <|> right <|> assumption}
+
+#check L7
+
+
+lemma L8 : ∀ (p q r:Prop), r → p ∨ q ∨ r :=
+  assume p q r H, by repeat {{left, assumption} <|> right <|> assumption}
+
+#check L8
+
+meta def my_tac : tactic unit :=
+  `[ repeat { {left, assumption} <|> right <|> assumption}]
+
+#check my_tac
+
+
+lemma L9 : ∀ (p q r:Prop), p → p ∨ q ∨ r :=
+  assume p q r H, by my_tac
+
+#check L9
+
+
+lemma L10 : ∀ (p q r:Prop), q → p ∨ q ∨ r :=
+  assume p q r H, by my_tac
+
+#check L10
+
+lemma L11 : ∀ (p q r:Prop), r → p ∨ q ∨ r :=
+  assume p q r H, by my_tac
+
+#check L11
+
+
+lemma L12 : ∀ (p q r:Prop), p → q → r → p ∧ q ∧ r :=
+  assume p q r Hp Hq Hr, by split; try {split}; assumption
+
+#check L12
+
+
+lemma L13 : ∀ (p q r:Prop), p → q → r → p ∧ q ∧ r :=
+  assume p q r Hp Hq Hr, by
+    begin
+      split,
+      all_goals {try {split}},
+      all_goals {assumption}
+    end
+
+#check L13
+
+
+lemma L14 : ∀ (p q r:Prop), p → q → r → p ∧ q ∧ r :=
+  assume p q r Hp Hq Hr, by
+    begin
+      split,
+      any_goals {split},
+      any_goals {assumption}
+    end
+
+#check L14
+
+
+lemma L15 : ∀ (p q r:Prop), p → q → r → p ∧ ((p ∧ q) ∧ r) ∧ (q ∧ r ∧ p) :=
+  assume p q r Hp Hq Hr,
+    begin
+      repeat {any_goals {split}},
+      all_goals {assumption}
+    end
+
+#check L15
+
+
+lemma L16 : ∀ (p q r:Prop), p → q → r → p ∧ ((p ∧ q) ∧ r) ∧ (q ∧ r ∧ p) :=
+  assume p q r Hp Hq Hr,
+    begin
+      repeat {any_goals {split <|> assumption}}
+    end
+
+#check L16
