agda/plfa/bin.agda
@@ -5,6 +5,7 @@ open Eq using (_≡_; refl; cong; sym)
 open Eq.≡-Reasoning using (begin_; _≡⟨⟩_; _≡⟨_⟩_;_∎)
 open import Data.Nat using (ℕ; zero; suc; _+_; _*_; _∸_;_^_) -- \.-
 
+open import induction
 
 data Bin : Set where
   ⟨⟩ : Bin
@@ -34,8 +35,8 @@ to (suc n) = inc (to n)
 
 from : Bin → ℕ
 from ⟨⟩    = 0
-from (n O) = 2 * (from n)
-from (n I) = 2 * (from n) + 1
+from (b O) = 2 * (from b)
+from (b I) = suc (2 * (from b))
 
 from-inc : ∀ (b : Bin) → from (inc b) ≡ suc (from b)
 from-inc ⟨⟩ = refl
@@ -45,12 +46,49 @@ from-inc (b O) =
     ≡⟨⟩
     from (b I)
     ≡⟨⟩
-    2 * (from b) + 1
+    suc (2 * (from b))
     ≡⟨⟩
-    {!!}
-from-inc (b I) = {!!}
+    suc (from (b O))
+    ∎
+from-inc (b I) =
+  begin
+    from (inc (b I))
+    ≡⟨⟩
+    from (inc b O)
+    ≡⟨⟩
+    2 * (from (inc b))
+    ≡⟨ cong (2 *_) (from-inc b) ⟩
+    2 * (suc (from b))
+    ≡⟨⟩
+    suc (from b) + 1 * (suc (from b))
+    ≡⟨⟩
+    suc (from b + 1 * (suc (from b)))
+    ≡⟨⟩
+    suc (from b + (suc (from b) + zero))
+    ≡⟨ cong (λ k → suc (from b + k)) (+-identity-r (suc (from b))) ⟩
+    suc (from b + suc (from b))
+    ≡⟨ cong suc (+-suc (from b) (from b)) ⟩
+    suc (suc (from b + from b))
+    ≡⟨ sym (cong (λ k → suc (suc (from b + k))) (+-identity-r (from b))) ⟩
+    suc (suc (from b + (from b + zero)))
+    ≡⟨⟩
+    suc (suc (2 * from b))
+    ≡⟨⟩
+    suc (from (b I))
+    ∎
+
+n0 : ℕ
+n0 = from ⟨⟩
+
+n1 : ℕ
+n1 = from (⟨⟩ O)
 
 
-
-
+{-
+-- not true: to (from ⟨⟩) = ⟨⟩ O ≠ ⟨⟩ , but both ⟨⟩ O and ⟨⟩ represent 0.
+to-from : ∀ (b : Bin) → to (from b) ≡ b
+to-from ⟨⟩ = {!!}
+to-from (b O) = {!!}
+to-from (b I) = {!!}
+-}
 
